updated duality proofs to be consistent with polymorphic version of model satisfaction

equational_theories/Duality.lean
@@ -1,7 +1,16 @@
+import equational_theories.Completeness
 import equational_theories.Conjecture
 import equational_theories.FreeMagma
 
 universe u
+
+def dualizeLaw {α : Type} (law : MagmaLaw α) : MagmaLaw α :=
+  dualizeTree law.lhs ≃ dualizeTree law.rhs
+
+theorem DualizeLawIsInvolution {α : Type} (law : MagmaLaw α) : dualizeLaw (dualizeLaw law) = law :=
+  Eq.trans
+    (congrArg (fun expr ↦ expr ≃ (dualizeTree $ dualizeTree law.rhs)) (DualizeTreeIsInvolution law.lhs))
+    (congrArg (fun expr ↦ law.lhs ≃ expr) (DualizeTreeIsInvolution law.rhs))
 
 inductive DualMagma (α : Type u) [Magma α]
   | DualWrap : α → DualMagma α
@@ -22,8 +31,8 @@ theorem DualMapIsAntihomomorphism (G : Type u) [Magma G] : ∀ x y : G, dualWrap
 theorem DualMapCancellable (G : Type u) [Magma G] : ∀ x y : G, dualWrap x = dualWrap y → x = y :=
   fun _ _ eq ↦ congrArg dualUnwrap eq
 
-theorem EvalReversedInDualMagma (G : Type u) [Magma G]
-  (expr : FreeMagma Nat) (sub : Nat → G) : dualWrap (evalInMagma sub expr) = evalInMagma (dualWrap ∘ sub) (dualizeTree expr) :=
+theorem EvalReversedInDualMagma {α : Type} (G : Type u) [Magma G]
+  (expr : FreeMagma α) (sub : α → G) : dualWrap (evalInMagma sub expr) = evalInMagma (dualWrap ∘ sub) (dualizeTree expr) :=
   match expr with
   | FreeMagma.Leaf n => Eq.refl (dualWrap $ sub n)
   | FreeMagma.Fork leftExpr rightExpr => by
@@ -39,30 +48,30 @@ theorem EvalReversedInDualMagma (G : Type u) [Magma G]
       (congrArg (fun t ↦ (evalInMagma subd (dualizeTree rightExpr)) ∘ t) leftCase)
       decompDualEval
 
-theorem EvalPreservedInDoubleDualMagma (G : Type u) [Magma G]
-  (expr : FreeMagma Nat) (sub : Nat → G) : dualWrap (dualWrap (evalInMagma sub expr)) = evalInMagma (dualWrap ∘ (dualWrap ∘ sub)) expr :=
+theorem EvalPreservedInDoubleDualMagma {α : Type} (G : Type u) [Magma G]
+  (expr : FreeMagma α) (sub : α → G) : dualWrap (dualWrap (evalInMagma sub expr)) = evalInMagma (dualWrap ∘ (dualWrap ∘ sub)) expr :=
   Eq.trans
     (congrArg dualWrap (EvalReversedInDualMagma G expr sub)) $ Eq.trans
     (EvalReversedInDualMagma (DualMagma G) (dualizeTree expr) (dualWrap ∘ sub))
     (congrArg (evalInMagma (dualWrap ∘ dualWrap ∘ sub)) (DualizeTreeIsInvolution expr))
 
-theorem DualizeLawFromMagma (G : Type u) [Magma G]
-  (law : EquationLaw) (pf : G ⊨ law) : DualMagma G ⊨ dualizeLaw law := by
+theorem DualizeLawFromMagma {α : Type} (G : Type) [Magma G]
+  (law : MagmaLaw α) (pf : G ⊧ law) : DualMagma G ⊧ dualizeLaw law := by
   intro subd
   let sub := dualUnwrap ∘ subd
   let subd' := dualWrap ∘ sub
   have subEquiv : subd' = subd := funext (fun n ↦ congrArg dualWrap (refl _))
   have eq : evalInMagma sub law.1 = evalInMagma sub law.2 := pf sub
   have eqd' : evalInMagma subd' (dualizeTree law.1) = evalInMagma subd' (dualizeTree law.2) := Eq.trans
-    (Eq.symm $ EvalReversedInDualMagma G law.1 sub) $ Eq.trans
+    (Eq.symm $ EvalReversedInDualMagma G law.lhs sub) $ Eq.trans
     (congrArg dualWrap eq)
-    (EvalReversedInDualMagma G law.2 sub)
+    (EvalReversedInDualMagma G law.rhs sub)
   have eqd : evalInMagma subd (dualizeTree law.1) = evalInMagma subd (dualizeTree law.2) :=
     Eq.rec (motive := fun f _ ↦ evalInMagma f (dualizeTree law.1) = evalInMagma f (dualizeTree law.2)) eqd' subEquiv
   exact eqd
 
-theorem UndualizeLawFromDualMagma (G : Type u) [Magma G]
-  (law : EquationLaw) (dualPf : DualMagma G ⊨ dualizeLaw law) : G ⊨ law := by
+theorem UndualizeLawFromDualMagma {α : Type} (G : Type) [Magma G]
+  (law : MagmaLaw α) (dualPf : DualMagma G ⊧ dualizeLaw law) : G ⊧ law := by
   intro sub
   let subd := dualWrap ∘ sub
   have dualLawSpecialized : evalInMagma subd (dualizeTree law.1) = evalInMagma subd (dualizeTree law.2) := dualPf subd
@@ -71,18 +80,18 @@ theorem UndualizeLawFromDualMagma (G : Type u) [Magma G]
     dualLawSpecialized
     (Eq.symm $ EvalReversedInDualMagma G law.2 sub)))
 
-theorem DualizeLawFromDualMagma (G : Type u) [Magma G]
-  (law : EquationLaw) (dualPf : DualMagma G ⊨ law) : G ⊨ dualizeLaw law := by
-  have satDoubleDual : DualMagma G ⊨ dualizeLaw (dualizeLaw law) := Eq.ndrec dualPf (Eq.symm $ DualizeLawIsInvolution law)
+theorem DualizeLawFromDualMagma {α : Type} (G : Type) [Magma G]
+  (law : MagmaLaw α) (dualPf : DualMagma G ⊧ law) : G ⊧ dualizeLaw law := by
+  have satDoubleDual : DualMagma G ⊧ dualizeLaw (dualizeLaw law) := Eq.ndrec dualPf (Eq.symm $ DualizeLawIsInvolution law)
   exact (UndualizeLawFromDualMagma G (dualizeLaw law) satDoubleDual)
 
 theorem DualizeEquationLawImplication
-  (law1 law2 : EquationLaw) (imp : ∀ (G : Type u) [Magma G], G ⊨ law1 → G ⊨ law2)
-  : (∀ (H : Type u) [Magma H], H ⊨ dualizeLaw law1 → H ⊨ dualizeLaw law2) := by
+  {α : Type} (law1 law2 : MagmaLaw α) (imp : ∀ (G : Type) [Magma G], G ⊧ law1 → G ⊧ law2)
+  : (∀ (H : Type) [Magma H], H ⊧ dualizeLaw law1 → H ⊧ dualizeLaw law2) := by
   intros G _ satDualLaw1
-  have dualSatLaw1 : DualMagma G ⊨ law1 := Eq.ndrec
-    (motive := fun l ↦ DualMagma G ⊨ l)
+  have dualSatLaw1 : DualMagma G ⊧ law1 := Eq.ndrec
+    (motive := fun (l : MagmaLaw α) ↦ DualMagma G ⊧ l)
     (DualizeLawFromMagma G (dualizeLaw law1) $ satDualLaw1)
     (DualizeLawIsInvolution law1)
-  have dualSatLaw2 : DualMagma G ⊨ law2 := imp (DualMagma G) dualSatLaw1
+  have dualSatLaw2 : DualMagma G ⊧ law2 := imp (DualMagma G) dualSatLaw1
   exact (DualizeLawFromDualMagma G law2 dualSatLaw2)
